queue-basic: add size

misc/queue-basic-known.bpl
@@ -141,12 +141,13 @@ var {:layer 0, 1} head: Ref;
 var {:layer 0, 1} tail: Ref;
 
 
-function {:inline} Inv(queueFP: [Ref]bool, head: Ref, tail: Ref, next: [Ref]Ref) : (bool)
+function {:inline} Inv(queueFP: [Ref]bool, UsedFP: [Ref]bool, head: Ref, tail: Ref, next: [Ref]Ref) : (bool)
 {
   Btwn(next, head, head, null)
     && Btwn(next, head, tail, null)
     && Equal(BtwnSet(next, head, null),
              Union(Singleton(null), queueFP))
+    && (forall x: Ref :: Btwn(next, x, x, head) ==> UsedFP[x])
     && tail != null
     && known(head) && known(tail) && known(null) && knownF(next)
 }
@@ -240,32 +241,32 @@ procedure {:atomic} {:layer 2} atomic_pop() returns (t: Ref)
 }
 
 procedure {:yields} {:layer 1} {:refines "atomic_pop"} pop() returns (h: Ref)
-requires {:layer 1} Inv(queueFP, head, tail, next);
-ensures {:layer 1} Inv(queueFP, head, tail, next);
+requires {:layer 1} Inv(queueFP, UsedFP, head, tail, next);
+ensures {:layer 1} Inv(queueFP, UsedFP, head, tail, next);
 {
   var g: bool;
   var t, x: Ref;
 
   yield;
-  assert {:layer 1} Inv(queueFP, head, tail, next);
+  assert {:layer 1} Inv(queueFP, UsedFP, head, tail, next);
   while (true)
-    invariant {:layer 1} Inv(queueFP, head, tail, next);
+    invariant {:layer 1} Inv(queueFP, UsedFP, head, tail, next);
   {
     call h := Readhead();
     yield;
-    assert {:layer 1} Inv(queueFP, head, tail, next);
+    assert {:layer 1} Inv(queueFP, UsedFP, head, tail, next);
     assert {:layer 1} h == head || UsedFP[h];
 
     call t := Readtail();
     yield;
-    assert {:layer 1} Inv(queueFP, head, tail, next);
+    assert {:layer 1} Inv(queueFP, UsedFP, head, tail, next);
     assert {:layer 1} h == head || UsedFP[h];
     assert {:layer 1} (h == head && h != t ==> head != tail);
 
     if (h != t) {
       call x := Load(h);
       yield;
-      assert {:layer 1} Inv(queueFP, head, tail, next);
+      assert {:layer 1} Inv(queueFP, UsedFP, head, tail, next);
       assert {:layer 1} h == head || UsedFP[h];
       assert {:layer 1} (h == head && h != t ==> x == next[head]);
       assert {:layer 1} (h == head && h != t ==> head != tail);
@@ -276,10 +277,10 @@ ensures {:layer 1} Inv(queueFP, head, tail, next);
       }
     }
     yield;
-    assert {:layer 1} Inv(queueFP, head, tail, next);
+    assert {:layer 1} Inv(queueFP, UsedFP, head, tail, next);
   }
   yield;
-  assert {:expand} {:layer 1} Inv(queueFP, head, tail, next);
+  assert {:expand} {:layer 1} Inv(queueFP, UsedFP, head, tail, next);
 }
 
 
@@ -295,38 +296,42 @@ procedure {:atomic} {:layer 2} atomic_push(x: Ref,
 }
 
 procedure {:yields} {:layer 1} {:refines "atomic_push"} push(x: Ref, {:linear_in "FP"} x_Heap: [Ref]bool)
-  requires {:layer 1} x_Heap[x] && next[x] == null;
-  requires {:layer 1} Inv(queueFP, head, tail, next);
-  ensures {:layer 1} Inv(queueFP, head, tail, next);
+  requires {:layer 1} x_Heap[x] && next[x] == null && !Btwn(next, head, x, null);
+  requires {:layer 1} Inv(queueFP, UsedFP, head, tail, next);
+  ensures {:layer 1} Inv(queueFP, UsedFP, head, tail, next);
 {
   var t, tn: Ref;
   var g: bool;
   var {:linear "FP"} t_Heap: [Ref]bool;
 
   yield;
-  assert {:layer 1} Inv(queueFP, head, tail, next);
+  assert {:layer 1} Inv(queueFP, UsedFP, head, tail, next);
+  assert {:layer 1} !Btwn(next, head, x, null);
   assert {:layer 1} x_Heap[x] && next[x] == null;
   t_Heap := x_Heap;
   while (true)
-    invariant {:layer 1} Inv(queueFP, head, tail, next);
+    invariant {:layer 1} Inv(queueFP, UsedFP, head, tail, next);
+    invariant {:layer 1} !Btwn(next, head, x, null);
     invariant {:layer 1} t_Heap == x_Heap;
     invariant {:layer 1} x_Heap[x] && next[x] == null;
   {
     call t := Readtail();
     yield;
-    assert {:layer 1} Inv(queueFP, head, tail, next);
+    assert {:layer 1} Inv(queueFP, UsedFP, head, tail, next);
+    assert {:layer 1} !Btwn(next, head, x, null);
     assert {:layer 1} t_Heap == x_Heap;
     assert {:layer 1} x_Heap[x] && next[x] == null;
-    assert {:layer 1} t != null && (Btwn(next, head, t, null)
+    assert {:layer 1} known(t) && t != null && (Btwn(next, head, t, null)
       || UsedFP[t]);
     assert {:layer 1} next[t] == null ==> t == tail;
 
     call tn := Load(t);
     yield;
-    assert {:layer 1} Inv(queueFP, head, tail, next);
+    assert {:layer 1} Inv(queueFP, UsedFP, head, tail, next);
+    assert {:layer 1} !Btwn(next, head, x, null);
     assert {:layer 1} t_Heap == x_Heap;
     assert {:layer 1} x_Heap[x] && next[x] == null;
-    assert {:layer 1} t != null && (Btwn(next, head, t, null)
+    assert {:layer 1} known(t) && t != null && (Btwn(next, head, t, null)
       || UsedFP[t]);
     assert {:layer 1} next[t] == null ==> t == tail;
 
@@ -337,50 +342,50 @@ procedure {:yields} {:layer 1} {:refines "atomic_push"} push(x: Ref, {:linear_in
       }
     } // TODO else cas tail
     yield;
-    assert {:layer 1} Inv(queueFP, head, tail, next);
+    assert {:layer 1} Inv(queueFP, UsedFP, head, tail, next);
+    assert {:layer 1} !Btwn(next, head, x, null);
     assert {:layer 1} t_Heap == x_Heap;
     assert {:layer 1} x_Heap[x] && next[x] == null;
   }
   yield;
-  assert {:expand} {:layer 1} Inv(queueFP, head, tail, next);
+  assert {:expand} {:layer 1} Inv(queueFP, UsedFP, head, tail, next);
 }
 
-/*
 
 procedure {:atomic} {:layer 2} atomic_size() returns (x: int)
 {}
 
 procedure {:yields} {:layer 1} {:refines "atomic_size"} size() returns (x: int)
-requires {:layer 1} Inv(queueFP, head, tail, next);
-ensures {:layer 1} Inv(queueFP, head, tail, next);
+requires {:layer 1} Inv(queueFP, UsedFP, head, tail, next);
+ensures {:layer 1} Inv(queueFP, UsedFP, head, tail, next);
 {
   var c: Ref;
+  var c1: Ref;
 
   yield;
-  assert {:layer 1} Inv(queueFP, head, tail, next);
+  assert {:layer 1} Inv(queueFP, UsedFP, head, tail, next);
 
   x := 0;
   call c := Readhead();
 
   yield;
-  assert {:layer 1} Inv(queueFP, head, tail, next);
-  assert {:layer 1} (UsedFP[c] && Btwn(next, c, c, head))
-    || Btwn(next, head, c, null);
+  assert {:layer 1} Inv(queueFP, UsedFP, head, tail, next);
+  assert {:layer 1} known(c) && ((UsedFP[c] && Btwn(next, c, c, head))
+    || Btwn(next, head, c, null));
 
   while (c != null)
-    invariant {:layer 1} Inv(queueFP, head, tail, next);
-    invariant {:layer 1} (UsedFP[c] && Btwn(next, c, c, head))
-      || Btwn(next, head, c, null);
+    invariant {:layer 1} Inv(queueFP, UsedFP, head, tail, next);
+    invariant {:layer 1} known(c) && ((UsedFP[c] && Btwn(next, c, c, head))
+      || Btwn(next, head, c, null));
   {
     x := x + 1;
-    call c := Load(c); // TODO: load doesn't return next if not in dom!?
+    call c1 := Load(c);
     yield;
-    assert {:layer 1} Inv(queueFP, head, tail, next);
-    assert {:layer 1} (UsedFP[c] && Btwn(next, c, c, head))
-                        || Btwn(next, head, c, null); // AtomicTransferToqueue breaks this, but it shouldn't!?
+    assert {:layer 1} Inv(queueFP, UsedFP, head, tail, next);
+    assert {:layer 1} known(c) && ((UsedFP[c] && Btwn(next, c, c, head))
+                        || Btwn(next, head, c, null));
   }
   yield;
-  assert {:layer 1} Inv(queueFP, head, tail, next);
+  assert {:layer 1} Inv(queueFP, UsedFP, head, tail, next);
   return;
 }
-*/
